proof/agp32CorrectScript.sml
@@ -2,28 +2,67 @@ open hardwarePreamble agp32StateTheory agp32EnvironmentTheory agp32ProcessorTheo
 
 val _ = new_theory "agp32Correct";
 
+(* Special variables used in theorems:
+   I: scheduling function.
+   C: cache oracle.
+ *)
+
 val _ = prefer_num ();
 val _ = guess_lengths ();
 
-(* I: scheduling function
-   C: cache oracle
- *)
+Theorem agp32_Init_implies_Rel:
+  !k fext fbits s a I.
+    k >= 1 ==>
+    k <= 5 ==>
+    s = agp32 fext fbits ==>
+    is_mem fext_accessor_circuit s fext ==>
+    is_acc accelerator_f s ==>
+    is_interrupt_interface fext_accessor_circuit s fext ==>
+    Init (fext 0) (s 0) a ==>
+    I(k,0) = 0 ==>
+    Rel (fext 0) (s 0) k a 0
+Proof
+  rpt strip_tac >>
+  fs [Init_def,Rel_def] >>
+  Cases_on `k = 1` >-
+   (fs [] >> cheat) >>
+  Cases_on `k = 2` >-
+   (fs [] >> cheat) >>
+  Cases_on `k = 3` >-
+   (fs [] >> cheat) >>
+  Cases_on `k = 4` >-
+   (fs [] >> cheat) >>
+  Cases_on `k = 5` >-
+   (fs [] >> cheat) >> fs []
+QED
+
 Theorem agp32_Rel_ag32_correct:
   !(k:num) fext fbits s a (t:num) i I C.
+    k >= 1 ==>
+    k <= 5 ==>
     s = agp32 fext fbits ==>
-    SC_self_mod (s t) ==>
+    (!t. SC_self_mod (s t)) ==>
     is_mem fext_accessor_circuit s fext ==>
     is_acc accelerator_f s ==>
     is_interrupt_interface fext_accessor_circuit s fext ==>
     (* cache oracle can introduce hit/miss *)
-    (C (s t).data_addr (s t).data_wstrb (s t).data_wdata (s t).command (s t).PC <=> (fext t).ready) ==>
+    (!t. C (s t).data_addr (s t).data_wstrb (s t).data_wdata (s t).command (s t).PC <=> (fext t).ready) ==>
     Init (fext 0) (s 0) a ==>
     (** properties of scheduling function I **)
-    (enable_stg k (s t) ==> I(k,t) = I(k-1,t) - 1) ==>
+    (!t k. enable_stg k (s t) ==> I(k,t) = I(k,t-1) + 1) ==>
+    I(k,0) = 0 ==>
     I(k,t) = i ==>
     Rel (fext t) (s t) k a i
 Proof
-  REPEAT STRIP_TAC >> cheat
+  rpt strip_tac >>
+  Induct_on `t` >>
+  rpt strip_tac >-
+   METIS_TAC [agp32_Init_implies_Rel] >>
+  fs [Init_def,Rel_def] >>
+  Cases_on `k = 1` >-
+   (** IF stage **)
+   (fs [] >> rw [] >> cheat) >>
+  cheat
 QED
 
 val _ = export_theory ();
